Lose has_mem instance for mypath

src/graph_theory/path.lean
@@ -7,6 +7,8 @@ namespace simple_graph
 
     def mypath (G : simple_graph V) := walk G
 
+    instance (G : simple_graph V) (x y : V) : has_mem V (walk G x y) := ⟨λ z p, z ∈ p.support⟩
+
     infix ` · `:50 := λ p h, walk.append p (walk.cons h walk.nil)
     infixr ` :: `  := walk.cons
     infix ` ++ `   := walk.append
@@ -15,41 +17,37 @@ namespace simple_graph
         open mypath walk
 
         variables {G G₁ G₂ : simple_graph V} {u v x y z : V} {e : edge G}
-        variables {p : mypath G x y} {p' : mypath G y z} {p'' : mypath G z u} {h : G.adj y z} {h' : G.adj u x} {h'' : G.adj z v}
+        variables {p : walk G x y} {p' : walk G y z} {p'' : walk G z u} {h : G.adj y z} {h' : G.adj u x} {h'' : G.adj z v}
 
-        @[simp] def mem    (z : V) (p : mypath G x y)             := z ∈ p.support
         @[simp] def size   (p : mypath G x y)                     := p.length
         @[simp] def rev    (p : mypath G x y)                     := walk.reverse p
-        @[simp] def nodup  (p : mypath G x y)                     := p.support.nodup
+        @[simp] def nodup  (p : walk G x y)                       := p.support.nodup
 
-        instance : has_mem V (walk G x y) := ⟨mem⟩
-        instance : has_mem V (mypath G x y) := ⟨mem⟩
         instance : has_sizeof (mypath G x y) := ⟨size⟩
 
-        @[simp] def myedges : Π {x y : V}, mypath G x y -> list (edge G)
+        @[simp] def myedges : Π {x y : V}, walk G x y -> list (edge G)
             | _ _ nil             := []
             | _ _ (walk.cons h p) := ⟨h⟩ :: myedges p
 
-        @[simp] lemma mem_point'   :   u ∈ (@nil _ G x) <-> u = x            := list.mem_singleton
-        @[simp] lemma size_rev     :       size (rev p)  =  size p           := length_reverse p
-        @[simp] lemma concat_rev   :      rev (p ++ p')  =  rev p' ++ rev p  := reverse_append p p'
-        @[simp] lemma size_concat  :     size (p ++ p')  =  size p + size p' := length_append p p'
-        @[simp] lemma concat_assoc :   (p ++ p') ++ p''  =  p ++ (p' ++ p'') := (append_assoc p p' p'').symm
+        @[simp] lemma mem_point'   : u ∈ (@nil _ G x).support <-> u = x                          := list.mem_singleton
+        @[simp] lemma size_rev     :             size (rev p)  =  size p                         := length_reverse p
+        @[simp] lemma concat_rev   :            rev (p ++ p')  =  rev p' ++ rev p                := reverse_append p p'
+        @[simp] lemma size_concat  :           size (p ++ p')  =  size p + size p'               := length_append p p'
+        @[simp] lemma concat_assoc :         (p ++ p') ++ p''  =  p ++ (p' ++ p'')               := (append_assoc p p' p'').symm
+        @[simp] lemma mem_concat   :    u ∈ (p ++ p') <-> u ∈ p ∨ u ∈ p' := mem_support_append_iff p p'
 
-        lemma mem_tail : y ∈ p := end_mem_support _
-        lemma mem_head : x ∈ p := start_mem_support _
+        lemma mem_tail : y ∈ p.support := end_mem_support _
+        lemma mem_head : x ∈ p.support := start_mem_support _
 
-        lemma point_of_size_0 : p.size = 0 -> x = y := by { intro h, cases p, refl, contradiction }
+        lemma point_of_size_0 : p.length = 0 -> x = y := by { intro h, cases p, refl, contradiction }
 
-        @[simp] lemma mem_concat : u ∈ append p p' <-> u ∈ p ∨ u ∈ p' := mem_support_append_iff p p'
-
-        lemma mem_edges : e ∈ p.myedges -> e.x ∈ p ∧ e.y ∈ p
+        lemma mem_edges : e ∈ myedges p -> e.x ∈ p.support ∧ e.y ∈ p.support
             := by { induction p with u u v w h p ih; simp, intro h', cases h',
-                { subst e, split, exact mem_head, right, exact mem_head },
+                { subst e, split, left, refl, right, exact mem_head },
                 { specialize ih h', exact ⟨or.inr ih.1, or.inr ih.2⟩ }
             }
 
-        lemma mem_of_edges (h : 0 < p.size) : u ∈ p.support <-> ∃ e ∈ p.myedges, u ∈ edge.ends e
+        lemma mem_of_edges (h : 0 < p.length) : u ∈ p.support <-> ∃ e ∈ myedges p, u ∈ edge.ends e
             := by { induction p with u u v w h p ih, { simp at h, contradiction }, clear h,
                 cases nat.eq_zero_or_pos (size p), { cases p, simp, simp at h_1, contradiction },
                 specialize ih h_1, clear h_1, simp at ih, split; simp,
@@ -60,16 +58,16 @@ namespace simple_graph
                         (λ e he h1, or.inr (ih.mpr ⟨e,he,h1⟩))⟩,
             }
 
-        lemma nodup_rev : nodup p -> nodup p.rev
-            := by { unfold nodup, unfold rev, rw (support_reverse p), exact list.nodup_reverse.mpr }
+        lemma nodup_rev : p.support.nodup -> p.reverse.support.nodup
+            := by { rw (support_reverse p), exact list.nodup_reverse.mpr }
 
-        lemma nodup_concat : nodup (append p p') <-> nodup p ∧ nodup p' ∧ (∀ u, u ∈ p -> u ∈ p' -> u = y)
+        lemma nodup_concat : nodup (append p p') <-> nodup p ∧ nodup p' ∧ (∀ u, u ∈ p.support -> u ∈ p'.support -> u = y)
             := by { induction p with a a b c h q ih; simp, push_neg, split,
-                { rintros ⟨⟨h1,h2⟩,h3⟩, replace ih := ih.mp h3, refine ⟨⟨h1,ih.1⟩,ih.2.1,λ u h4 h5, _⟩,
-                    cases h4, rw h4 at h5, contradiction, exact ih.2.2 u h4 h5 },
-                { rintros ⟨⟨h1,h2⟩,h3,h4⟩, refine ⟨⟨h1,_⟩,_⟩,
-                    intro h5, apply h1, rw h4 a mem_head h5, exact mem_tail,
-                    refine ih.mpr ⟨h2,h3,_⟩, intros u hu h'u, refine h4 u (or.inr hu) h'u } }
+                { rintros ⟨⟨h1,h2⟩,h3⟩, replace ih := ih.mp h3, refine ⟨⟨h1,ih.1⟩,ih.2.1,_,λ u h4 h5, _⟩,
+                    intro, contradiction, exact ih.2.2 u h4 h5 },
+                { rintros ⟨⟨h1,h2⟩,h3,h4,h5⟩, refine ⟨⟨h1,_⟩,_⟩,
+                    intro h5, apply h1, rw h4 h5, exact mem_tail,
+                    refine ih.mpr ⟨h2,h3,_⟩, intros u hu h'u, exact h5 u hu h'u } }
 
         def path_from_subgraph (sub : ∀ {x y}, G₁.adj x y -> G₂.adj x y) : Π {x y : V}, mypath G₁ x y -> mypath G₂ x y
             | _ _ nil             := nil
